CellularAutomatas/results_unproven.lean
@@ -18,9 +18,9 @@ theorem exp_word_length_rt: ∃ C: CA_rt Unit, C.val.L = { w | ∃ n, w.length =
   sorry
 
 
-
-theorem linear_time_dead_border (C: CA_lt α): ∃ C': tCellAutomaton α, C'.dead C'.border ∧ C'.similar C := by
-  sorry
+-- TODO: Define tCellAutomaton.similar
+-- theorem linear_time_dead_border (C: CA_lt α): ∃ C': tCellAutomaton α, C'.dead C'.border ∧ C'.similar C := by
+--   sorry
 
 theorem const_speed_up: ℒ ({ C ∈ CA α | ∃ k, ∀ n, C.t n = n + k - 1 }) = ℒ (CA_rt α) := by
   sorry
